poST_utils/poST_expr_utils.thy
@@ -1,0 +1,15 @@
+theory poST_expr_utils
+  imports basic_poST_types_utils "~~/poST/poST_model/poST_expr"
+begin
+definition proc_status_is :: "proc_status \<Rightarrow> proc_status \<Rightarrow> bool" where
+"proc_status_is s1 s2 = 
+(case (s1,s2) of 
+  (proc_status.Active,proc_status.Active) \<Rightarrow> True |
+  (proc_status.Inactive,proc_status.Inactive) \<Rightarrow> True |
+  (proc_status.Stop,proc_status.Stop) \<Rightarrow> True |
+  (proc_status.Error,proc_status.Error) \<Rightarrow> True |
+  (proc_status.Stop,proc_status.Inactive) \<Rightarrow> True |
+  (proc_status.Error,proc_status.Inactive) \<Rightarrow> True |
+  (proc_status.Timeout _, proc_status.Inactive) \<Rightarrow> False |
+  (_,_) \<Rightarrow> False)"
+end
